$ [[a_1 = 0 , b_1 = frac(y_2 - 2 thin y_1 + y_0, 2 thin h^2) , c_1 = - frac(x_0 thin (2 thin y_2 - 4 thin y_1) + h thin y_2 - 4 thin h thin y_1 + (2 thin x_0 + 3 thin h) thin y_0, 2 thin h^2) , d_1 = frac(x_0 thin (h thin y_2 - 4 thin h thin y_1) + x_0^2 thin (y_2 - 2 thin y_1) + (x_0^2 + 3 thin h thin x_0 + 2 thin h^2) thin y_0, 2 thin h^2) , a_2 = 0 , b_2 = frac(y_2 - 2 thin y_1 + y_0, 2 thin h^2) , c_2 = - frac(x_0 thin (2 thin y_2 - 4 thin y_1) + h thin y_2 - 4 thin h thin y_1 + (2 thin x_0 + 3 thin h) thin y_0, 2 thin h^2) , d_2 = frac(x_0 thin (h thin y_2 - 4 thin h thin y_1) + x_0^2 thin (y_2 - 2 thin y_1) + (x_0^2 + 3 thin h thin x_0 + 2 thin h^2) thin y_0, 2 thin h^2)]] $
