\begin{equation}
	\left[ \left[ a_{1}=0 , b_{1}={\frac{y_{2}-2\,y_{1}+y_{0}}{2\,h^2}}
	, c_{1}=-{\frac{x_{0}\,\left(2\,y_{2}-4\,y_{1}\right)+h\,y_{2}-4\,h\,
	y_{1}+\left(2\,x_{0}+3\,h\right)\,y_{0}}{2\,h^2}} , d_{1}={\frac{
	x_{0}\,\left(h\,y_{2}-4\,h\,y_{1}\right)+x_{0}^2\,\left(y_{2}-2\,
	y_{1}\right)+\left(x_{0}^2+3\,h\,x_{0}+2\,h^2\right)\,y_{0}}{2
	\,h^2}} , a_{2}=0 , b_{2}={\frac{y_{2}-2\,y_{1}+y_{0}}{2\,h^2}} ,
	c_{2}=-{\frac{x_{0}\,\left(2\,y_{2}-4\,y_{1}\right)+h\,y_{2}-4\,h\,y_{1}+
	\left(2\,x_{0}+3\,h\right)\,y_{0}}{2\,h^2}} , d_{2}={\frac{x_{0}\,
	\left(h\,y_{2}-4\,h\,y_{1}\right)+x_{0}^2\,\left(y_{2}-2\,y_{1}
	\right)+\left(x_{0}^2+3\,h\,x_{0}+2\,h^2\right)\,y_{0}}{2\,h^2
	}} \right]  \right]
\end{equation}
